iris_heap_lang/lib/logatom_lock.v
@@ -18,14 +18,14 @@ From iris.prelude Require Import options.
 
 Inductive state := Free | Locked.
 
-Class lockG Σ := LockG { lock_tokG : ghost_varG Σ state }.
+Class alockG Σ := LockG { lock_tokG : ghost_varG Σ state }.
 Local Existing Instance lock_tokG.
-Definition lockΣ : gFunctors := #[ghost_varΣ state].
-Global Instance subG_lockΣ {Σ} : subG lockΣ Σ → lockG Σ.
+Definition alockΣ : gFunctors := #[ghost_varΣ state].
+Global Instance subG_alockΣ {Σ} : subG alockΣ Σ → alockG Σ.
 Proof. solve_inG. Qed.
 
 Section tada.
-  Context `{!heapGS Σ, !lockG Σ, !lock}.
+  Context `{!heapGS Σ, !alockG Σ, !lock, !lockG Σ}.
 
   Record tada_lock_name := TadaLockName {
     tada_lock_name_state : gname;
